{
    "default_step_(0)": {
        "step_name": "default_step_(0)",
        "prompt": "Complete: 1, 2, 5, 14, ...",
        "thinking": "
        {
            "default_step_(0)": {
                "step_name": "default_step_(0)",
                "prompt": "Complete: 1, 2, 5, 14, ...",
                "thinking": "This is a sequence: 1, 2, 5, 14, ...

        Let me try to find the pattern. 

        First, let me look at the differences between consecutive terms:
        2 - 1 = 1
        5 - 2 = 3
        14 - 5 = 9

        So the differences are 1, 3, 9, which looks like powers of 3: 3^0, 3^1, 3^2.

        Let me check if the original sequence follows a pattern related to powers of 3:

        First term: 1 = 1
        Second term: 2 = 1 + 3^0
        Third term: 5 = 1 + 3^0 + 3^1 = 1 + 1 + 3 = 5
        Fourth term: 14 = 1 + 3^0 + 3^1 + 3^2 = 1 + 1 + 3 + 9 = 14

        So it looks like the pattern is:
        a_1 = 1
        a_n = a_{n-1} + 3^{n-2} for n ≥ 2

        Let's verify this:
        a_1 = 1
        a_2 = a_1 + 3^0 = 1 + 1 = 2
        a_3 = a_2 + 3^1 = 2 + 3 = 5
        a_4 = a_3 + 3^2 = 5 + 9 = 14

        So the pattern works. The next term should be:
        a_5 = a_4 + 3^3 = 14 + 27 = 41

        But let me check if there are other patterns that might fit.

        Another approach: Let's see if there's a direct formula for the nth term.

        First term: 1
        Second term: 2 = 1 + 1
        Third term: 5 = 1 + 1 + 3
        Fourth term: 14 = 1 + 1 + 3 + 9

        This looks like 1 + sum of powers of 3 from 3^0 to 3^{n-2}.

        The sum of geometric series 3^0 + 3^1 + ... + 3^{n-2} is (3^{n-1} - 1)/2.

        So the formula might be: a_n = 1 + (3^{n-1} - 1)/2

        Let's check:
        a_1 = 1 + (3^0 - 1)/2 = 1 + 0 = 1 ✓
        a_2 = 1 + (3^1 - 1)/2 = 1 + 1 = 2 ✓
        a_3 = 1 + (3^2 - 1)/2 = 1 + 4 = 5 ✓
        a_4 = 1 + (3^3 - 1)/2 = 1 + 13 = 14 ✓

        This formula works! So the next term would be:
        a_5 = 1 + (3^4 - 1)/2 = 1 + (81 - 1)/2 = 1 + 40 = 41

        Hmm, wait, there's a problem. I made a mistake in my calculation of the sum of the geometric series. The correct formula for the sum of 3^0 + 3^1 + ... + 3^{n-2} is (3^{n-1} - 1)/(3-1) = (3^{n-1} - 1)/2.

        But this gives me the same answer, so I think I was on the right track.

        Let's double-check:
        a_1 = 1 (given)
        a_2 = 2 (given)
        a_3 = 5 (given)
        a_4 = 14 (given)
        a_5 = ?

        If a_n = 1 + (3^{n-1} - 1)/2, then:
        a_5 = 1 + (3^4 - 1)/2 = 1 + (81 - 1)/2 = 1 + 40 = 41

        Actually, let me try a different approach to confirm. Let's try to find a direct recursive formula.

        The differences between consecutive terms are 1, 3, 9, which are 3^0, 3^1, 3^2. So it seems like the difference between a_n and a_{n-1} is 3^{n-2}.

        So a_n = a_{n-1} + 3^{n-2}

        Starting with a_1 = 1:
        a_2 = a_1 + 3^0 = 1 + 1 = 2
        a_3 = a_2 + 3^1 = 2 + 3 = 5
        a_4 = a_3 + 3^2 = 5 + 9 = 14
        a_5 = a_4 + 3^3 = 14 + 27 = 41

        So the fifth term is 41.

        Wait, let me triple check this from scratch.

        The sequence is: 1, 2, 5, 14, ...

        First differences: 2-1=1, 5-2=3, 14-5=9

        These differences are: 1, 3, 9, which is 3^0, 3^1, 3^2

        So it seems the pattern is:
        a_1 = 1
        a_n = a_{n-1} + 3^{n-2} for n ≥ 2

        Let's verify:
        a_1 = 1 (given)
        a_2 = a_1 + 3^0 = 1 + 1 = 2 (matches given)
        a_3 = a_2 + 3^1 = 2 + 3 = 5 (matches given)
        a_4 = a_3 + 3^2 = 5 + 9 = 14 (matches given)

        So the next term is:
        a_5 = a_4 + 3^3 = 14 + 27 = 41

        Actually, I think I was wrong about the formula a_n = 1 + (3^{n-1} - 1)/2. Let me rethink this.

        If a_n = a_{n-1} + 3^{n-2}, then:
        a_1 = 1
        a_2 = a_1 + 3^0 = 1 + 1 = 2
        a_3 = a_2 + 3^1 = 2 + 3 = 5
        a_4 = a_3 + 3^2 = 5 + 9 = 14
        a_5 = a_4 + 3^3 = 14 + 27 = 41

        So the next term is 41.

        But let's try to find a direct formula. We have:
        a_1 = 1
        a_2 = 1 + 3^0
        a_3 = 1 + 3^0 + 3^1
        a_4 = 1 + 3^0 + 3^1 + 3^2

        So a_n = 1 + Σ(j=0 to n-2) 3^j

        This is 1 plus a geometric series with first term a=1 and common ratio r=3. The sum of a geometric series with n terms is (a(1-r^n))/(1-r). In our case:
        1 + 3^0 + 3^1 + ... + 3^{n-2} = 1 + (1(1-3^{n-1}))/(1-3) = 1 + (1-3^{n-1})/(-2) = 1 - (1-3^{n-1})/2 = 1 - 1/2 + 3^{n-1}/2 = 0.5 + 3^{n-1}/2

        So a_n = 0.5 + 3^{n-1}/2

        Let's check:
        a_1 = 0.5 + 3^0/2 = 0.5 + 0.5 = 1 ✓
        a_2 = 0.5 + 3^1/2 = 0.5 + 1.5 = 2 ✓
        a_3 = 0.5 + 3^2/2 = 0.5 + 4.5 = 5 ✓
        a_4 = 0.5 + 3^3/2 = 0.5 + 13.5 = 14 ✓

        So the formula is a_n = 0.5 + 3^{n-1}/2.

        For a_5, we get:
        a_5 = 0.5 + 3^4/2 = 0.5 + 81/2 = 0.5 + 40.5 = 41

        So the next term is 41.

        Hmm, let me check my calculation of the geometric series sum.

        a_n = 1 + 3^0 + 3^1 + ... + 3^{n-2}

        The sum of the geometric series 3^0 + 3^1 + ... + 3^{n-2} is (3^0(1-3^{n-1}))/(1-3) = (1-3^{n-1})/(-2) = (3^{n-1}-1)/2

        So a_n = 1 + (3^{n-1}-1)/2 = (2 + 3^{n-1} - 1)/2 = (1 + 3^{n-1})/2

        Let's check:
        a_1 = (1 + 3^0)/2 = (1 + 1)/2 = 1 ✓
        a_2 = (1 + 3^1)/2 = (1 + 3)/2 = 2 ✓
        a_3 = (1 + 3^2)/2 = (1 + 9)/2 = 5 ✓
        a_4 = (1 + 3^3)/2 = (1 + 27)/2 = 14 ✓

        So a_n = (1 + 3^{n-1})/2

        For a_5, we get:
        a_5 = (1 + 3^4)/2 = (1 + 81)/2 = 82/2 = 41

        So the next term is 41.

        I actually think I'm overthinking this. Let's go back to the recursion:
        a_1 = 1
        a_n = a_{n-1} + 3^{n-2} for n ≥ 2

        This gives:
        a_1 = 1
        a_2 = 1 + 1 = 2
        a_3 = 2 + 3 = 5
        a_4 = 5 + 9 = 14
        a_5 = 14 + 27 = 41

        So the next term is 41.

        Actually, let me try something else. Let's check if a polynomial fits the pattern.

        If we consider a cubic polynomial: a_n = an^3 + bn^2 + cn + d, we need to find a, b, c, d such that:
        a_1 = a(1)^3 + b(1)^2 + c(1) + d = 1
        a_2 = a(2)^3 + b(2)^2 + c(2) + d = 2
        a_3 = a(3)^3 + b(3)^2 + c(3) + d = 5
        a_4 = a(4)^3 + b(4)^2 + c(4) + d = 14

        This gives us a system of 4 equations with 4 unknowns. Let's solve it:

        For a_1:
        a + b + c + d = 1

        For a_2:
        8a + 4b + 2c + d = 2

        For a_3:
        27a + 9b + 3c + d = 5

        For a_4:
        64a + 16b + 4c + d = 14

        Let's subtract the first equation from the second:
        7a + 3b + c = 1

        Let's subtract the first equation from the third:
        26a + 8b + 2c = 4

        Let's subtract the first equation from the fourth:
        63a + 15b + 3c = 13

        Let's divide the second derived equation by 2:
        13a + 4b + c = 2

        Now, let's subtract the first derived equation from this:
        6a + b = 1

        Let's divide the third derived equation by 3:
        21a + 5b + c = 13/3

        Subtracting the first derived equation:
        14a + 2b = 10/3

        Multiplying the equation 6a + b = 1 by 2:
        12a + 2b = 2

        Subtracting this from 14a + 2b = 10/3:
        2a = 10/3 - 2 = 10/3 - 6/3 = 4/3
        So a = 2/3

        Substituting back:
        6(2/3) + b = 1
        4 + b = 1
        b = -3

        Now, let's find c:
        7(2/3) + 3(-3) + c = 1
        14/3 - 9 + c = 1
        14/3 - 27/3 + c = 1
        -13/3 + c = 1
        c = 1 + 13/3 = 3/3 + 13/3 = 16/3

        Now, let's find d using the first equation:
        a + b + c + d = 1
        2/3 + (-3) + 16/3 + d = 1
        2/3 - 9/3 + 16/3 + d = 1
        9/3 + d = 1
        d = 1 - 9/3 = 1 - 3 = -2

        So we have a = 2/3, b = -3, c = 16/3, d = -2.

        Let's check:
        a_1 = (2/3)(1)^3 + (-3)(1)^2 + (16/3)(1) + (-2) = 2/3 - 3 + 16/3 - 2 = 2/3 - 3 + 16/3 - 2 = (2 - 9 + 16 - 6)/3 = 3/3 = 1 ✓
        a_2 = (2/3)(2)^3 + (-3)(2)^2 + (16/3)(2) + (-2) = (2/3)(8) + (-3)(4) + (16/3)(2) + (-2) = 16/3 - 12 + 32/3 - 2 = (16 - 36 + 32 - 6)/3 = 6/3 = 2 ✓
        a_3 = (2/3)(3)^3 + (-3)(3)^2 + (16/3)(3) + (-2) = (2/3)(27) + (-3)(9) + (16/3)(3) + (-2) = 18 - 27 + 16 - 2 = 5 ✓
        a_4 = (2/3)(4)^3 + (-3)(4)^2 + (16/3)(4) + (-2) = (2/3)(64) + (-3)(16) + (16/3)(4) + (-2) = 128/3 - 48 + 64/3 - 2 = (128 - 144 + 64 - 6)/3 = 42/3 = 14 ✓

        So the polynomial a_n = (2/3)n^3 - 3n^2 + (16/3)n - 2 fits the given sequence.

        For a_5, we get:
        a_5 = (2/3)(5)^3 + (-3)(5)^2 + (16/3)(5) + (-2) = (2/3)(125) + (-3)(25) + (16/3)(5) + (-2) = 250/3 - 75 + 80/3 - 2 = (250 - 225 + 80 - 6)/3 = 99/3 = 33

        Hmm, that's not 41. Let me double-check my calculations.

        Actually, I made an error in solving the system of equations. Let me try a different approach.

        Using Newton's forward difference formula, we can find the polynomial that passes through the points (1,1), (2,2), (3,5), (4,14).

        First, we compute the forward differences:
        Δ^1: 1, 3, 9
        Δ^2: 2, 6
        Δ^3: 4

        Since Δ^3 is constant, a cubic polynomial will fit the data.

        Using the formula:
        a_n = a_1 + (n-1)Δa_1 + (n-1)(n-2)Δ^2a_1/2! + (n-1)(n-2)(n-3)Δ^3a_1/3!

        We have:
        a_1 = 1
        Δa_1 = 1
        Δ^2a_1 = 2
        Δ^3a_1 = 4

        So:
        a_n = 1 + (n-1)1 + (n-1)(n-2)2/2 + (n-1)(n-2)(n-3)4/6
            = 1 + (n-1) + (n-1)(n-2) + (n-1)(n-2)(n-3)2/3
            = 1 + (n-1) + (n-1)(n-2) + 2(n-1)(n-2)(n-3)/3

        For a_5, we get:
        a_5 = 1 + (5-1) + (5-1)(5-2) + 2(5-1)(5-2)(5-3)/3
            = 1 + 4 + 4*3 + 2*4*3*2/3
            = 1 + 4 + 12 + 16
            = 33

        But that doesn't match our previously computed a_5 = 41. Let me check if I've made a mistake.

        Actually, I've been thinking about this wrong. I need to revisit the original problem.

        The sequence is: 1, 2, 5, 14, ...

        I've established that the differences between consecutive terms are 1, 3, 9, which are 3^0, 3^1, 3^2.

        So the pattern is:
        a_1 = 1
        a_n = a_{n-1} + 3^{n-2} for n ≥ 2

        For a_5, we get:
        a_5 = a_4 + 3^3 = 14 + 27 = 41

        Let me also confirm the direct formula.

        a_1 = 1
        a_2 = 1 + 3^0
        a_3 = 1 + 3^0 + 3^1
        a_4 = 1 + 3^0 + 3^1 + 3^2

        So a_n = 1 + Σ(j=0 to n-2) 3^j

        This is 1 plus a geometric series with first term a=1 and common ratio r=3, with n-1 terms. The sum of a geometric series with n terms is a(1-r^n)/(1-r). In our case:
        Σ(j=0 to n-2) 3^j = (1-3^{n-1})/(1-3) = (1-3^{n-1})/(-2) = (3^{n-1}-1)/2

        So a_n = 1 + (3^{n-1}-1)/2 = (2 + 3^{n-1} - 1)/2 = (1 + 3^{n-1})/2

        Let's check:
        a_1 = (1 + 3^0)/2 = (1 + 1)/2 = 1 ✓
        a_2 = (1 + 3^1)/2 = (1 + 3)/2 = 2 ✓
        a_3 = (1 + 3^2)/2 = (1 + 9)/2 = 5 ✓
        a_4 = (1 + 3^3)/2 = (1 + 27)/2 = 14 ✓

        So a_n = (1 + 3^{n-1})/2

        For a_5, we get:
        a_5 = (1 + 3^4)/2 = (1 + 81)/2 = 82/2 = 41

        So the next term is 41.

        Let's revisit the polynomial approach. If the third difference is constant, a cubic polynomial should fit the data. But I might have made a mistake in computing the differences.

        Actual sequence: 1, 2, 5, 14
        First differences: 1, 3, 9
        Second differences: 2, 6
        Third differences: 4

        Hmm, the third difference is indeed 4. So a cubic polynomial should fit.

        Using the formula:
        a_n = 1 + (n-1) + (n-1)(n-2)/2*2 + (n-1)(n-2)(n-3)/6*4
            = 1 + (n-1) + (n-1)(n-2) + 2(n-1)(n-2)(n-3)/3

        For a_5, we get:
        a_5 = 1 + (5-1) + (5-1)(5-2) + 2(5-1)(5-2)(5-3)/3
            = 1 + 4 + 4*3 + 2*4*3*2/3
            = 1 + 4 + 12 + 16
            = 33

        But this doesn't match our previously computed a_5 = 41.

        Let me double-check the formula:
        a_n = a_1 + (n-1)Δa_1 + (n-1)(n-2)Δ^2a_1/2! + (n-1)(n-2)(n-3)Δ^3a_1/3!

        Let's compute the forward differences again:
        Sequence: 1, 2, 5, 14

        Δ^1: 1, 3, 9
        Δ^2: 2, 6
        Δ^3: 4

        So:
        a_n = 1 + (n-1)1 + (n-1)(n-2)2/2 + (n-1)(n-2)(n-3)4/6
            = 1 + (n-1) + (n-1)(n-2) + 2(n-1)(n-2)(n-3)/3

        Let's expand for a few values of n:
        a_1 = 1 + 0 + 0 + 0 = 1 ✓
        a_2 = 1 + 1 + 0 + 0 = 2 ✓
        a_3 = 1 + 2 + 2 + 0 = 5 ✓
        a_4 = 1 + 3 + 6 + 4 = 14 ✓

        So the formula seems correct.

        For a_5:
        a_5 = 1 + (5-1) + (5-1)(5-2)/2*2 + (5-1)(5-2)(5-3)/6*4
            = 1 + 4 + 4*3/2*2 + 4*3*2/6*4
            = 1 + 4 + 12 + 8
            = 25

        That's not 41 either.

        Let me double-check my calculations:
        (5-1)(5-2)/2*2 = 4*3/2*2 = 12
        (5-1)(5-2)(5-3)/6*4 = 4*3*2/6*4 = 24/6*4 = 4*4 = 16

        So, a_5 = 1 + 4 + 12 + 16 = 33

        I'm getting confused between 33 and 41.

        Let me go back to the recursive formula, which I'm confident about:
        a_1 = 1
        a_n = a_{n-1} + 3^{n-2} for n ≥ 2

        This gives:
        a_1 = 1
        a_2 = 1 + 3^0 = 1 + 1 = 2
        a_3 = 2 + 3^1 = 2 + 3 = 5
        a_4 = 5 + 3^2 = 5 + 9 = 14
        a_5 = 14 + 3^3 = 14 + 27 = 41

        So the next term should be 41.

        But I'm still puzzled by the polynomial. Let me try yet another approach.

        Actually, I believe the sequence is what's known as the \"3-Weak Schroeder numbers\". These numbers have a direct formula:
        a_n = (1 + 3^{n-1})/2

        This gives:
        a_1 = (1 + 3^0)/2 = (1 + 1)/2 = 1
        a_2 = (1 + 3^1)/2 = (1 + 3)/2 = 2
        a_3 = (1 + 3^2)/2 = (1 + 9)/2 = 5
        a_4 = (1 + 3^3)/2 = (1 + 27)/2 = 14
        a_5 = (1 + 3^4)/2 = (1 + 81)/2 = 41

        So the next term is 41.

        Let's also double-check the polynomial approach:

        Using the formula:
        a_n = a_1 + C(n-1,1)Δa_1 + C(n-1,2)Δ^2a_1 + C(n-1,3)Δ^3a_1

        Where C(n,k) is the binomial coefficient, \"n choose k\".

        We have:
        a_1 = 1
        Δa_1 = 1
        Δ^2a_1 = 2
        Δ^3a_1 = 4

        For a_5:
        a_5 = 1 + C(4,1)*1 + C(4,2)*2 + C(4,3)*4
            = 1 + 4*1 + 6*2 + 4*4
            = 1 + 4 + 12 + 16
            = 33

        Hmm, I'm still getting 33. Let me double-check the forward differences:

        Sequence: 1, 2, 5, 14
        First differences: 2-1=1, 5-2=3, 14-5=9
        Second differences: 3-1=2, 9-3=6
        Third differences: 6-2=4

        So the forward differences are correct.

        Let me check the formula again. For a cubic polynomial, we have:
        a_n = a_1 + C(n-1,1)Δa_1 + C(n-1,2)Δ^2a_1/2! + C(n-1,3)Δ^3a_1/3!

        For a_5:
        a_5 = 1 + C(4,1)*1 + C(4,2)*2/2! + C(4,3)*4/3!
            = 1 + 4*1 + 6*2/2 + 4*4/6
            = 1 + 4 + 6 + 8/3
            = 11 + 8/3
            = 33/3 + 8/3
            = 41/3

        That's not right. Let me check the formula one more time.

        Actually, I think I've been using the wrong formula. Let's use the forward difference formula directly.

        a_n = Σ(k=0 to n-1) [C(n-1, k) * Δ^k a_1]

        For a_5:
        a_5 = C(4,0)*a_1 + C(4,1)*Δa_1 + C(4,2)*Δ^2a_1 + C(4,3)*Δ^3a_1
            = 1*1 + 4*1 + 6*2 + 4*4
            = 1 + 4 + 12 + 16
            = 33

        But this still doesn't match our expected 41.

        Let me go back to the recursive formula, which I'm confident about:
        a_1 = 1
        a_n = a_{n-1} + 3^{n-2} for n ≥ 2

        This gives:
        a_1 = 1
        a_2 = 1 + 3^0 = 1 + 1 = 2
        a_3 = 2 + 3^1 = 2 + 3 = 5
        a_4 = 5 + 3^2 = 5 + 9 = 14
        a_5 = 14 + 3^3 = 14 + 27 = 41

        So the next term should be 41.

        Let's also validate the direct formula:
        a_n = (1 + 3^{n-1})/2

        For a_5:
        a_5 = (1 + 3^4)/2 = (1 + 81)/2 = 82/2 = 41

        So, a_5 = 41.

        Wait, I just realized a potential issue. I was assuming the formula is:
        a_n = a_1 + C(n-1,1)*Δa_1 + C(n-1,2)*Δ^2a_1 + C(n-1,3)*Δ^3a_1

        But the correct formula for Newton's forward difference is:
        a_n = a_1 + C(n-1,1)*Δa_1 + C(n-1,2)*Δ^2a_1/2! + C(n-1,3)*Δ^3a_1/3!

        So let's recalculate:
        a_5 = 1 + C(4,1)*1 + C(4,2)*2/2! + C(4,3)*4/3!
            = 1 + 4*1 + 6*2/2 + 4*4/6
            = 1 + 4 + 6 + 8/3
            = 11 + 8/3
            = 33 + 8/3
            = (99 + 8)/3
            = 107/3
            ≈ 35.67

        No, I'm making algebraic errors. Let me compute this carefully:
        a_5 = 1 + 4*1 + 6*2/2 + 4*4/6
            = 1 + 4 + 6 + 8/3
            = 1 + 4 + 6 + 2.67
            = 13.67

        This is still not 41.

        Actually, I'm now doubting the polynomial approach. Let's stick with the recursive formula which we've verified:
        a_1 = 1
        a_n = a_{n-1} + 3^{n-2} for n ≥ 2

        For a_5, we get:
        a_5 = a_4 + 3^3 = 14 + 27 = 41

        So the next term is 41.

        Actually, I think I've been overcomplicating this. The original pattern is:
        1, 2, 5, 14, ...

        Let's compute the differences:
        2-1=1, 5-2=3, 14-5=9

        The ratios between these differences: 3/1=3, 9/3=3

        So it seems like the differences are growing by a factor of 3.

        This gives us:
        a_1 = 1
        a_2 = 2
        a_3 = 5
        a_4 = 14
        a_5 = 14 + 9*3 = 14 + 27 = 41

        So the next term is 41.

        Let me try yet another formula approach. If a_n = a*3^n + b, then:
        a_1 = a*3^1 + b
        a_2 = a*3^2 + b
        a_3 = a*3^3 + b
        a_4 = a*3^4 + b

        From the first two equations:
        a_1 - a_2 = a*(3^1 - 3^2) = a*3^1*(1 - 3) = -2a*3^1
        1 - 2 = -2a*3^1
        -1 = -2a*3
        a = 1/(2*3) = 1/6

        Now, using the first equation:
        1 = a*3^1 + b
        1 = 1/6 * 3 + b
        1 = 1/2 + b
        b = 1/2

        So a_n = 3^n/6 + 1/2

        Let's check:
        a_1 = 3^1/6 + 1/2 = 3/6 + 1/2 = 1/2 + 1/2 = 1 ✓
        a_2 = 3^2/6 + 1/2 = 9/6 + 1/2 = 3/2 + 1/2 = 2 ✓
        a_3 = 3^3/6 + 1/2 = 27/6 + 1/2 = 9/2 + 1/2 = 5 ✓
        a_4 = 3^4/6 + 1/2 = 81/6 + 1/2 = 27/2 + 1/2 = 14 ✓

        For a_5:
        a_5 = 3^5/6 + 1/2 = 243/6 + 1/2 = 81/2 + 1/2 = 41

        So the next term is 41.

        Actually, I want to verify if this formula is equivalent to the one we had earlier:
        a_n = (1 + 3^{n-1})/2

        For a_n = 3^n/6 + 1/2, we have:
        a_n = 3^n/6 + 1/2 = 3^n/6 + 3/6 = (3^n + 3)/6 = (3^n + 3)/6 = (3*3^{n-1} + 3)/6 = 3(3^{n-1} + 1)/6 = (3^{n-1} + 1)/2

        So yes, they are equivalent.

        So, the next term in the sequence 1, 2, 5, 14, ... is 41.

        Actually, let me double-check the formula a_n = 3^n/6 + 1/2. I think I've been off by one in the exponent.

        If a_n = a*3^n + b, then:
        a_1 = a*3^1 + b = 1
        a_2 = a*3^2 + b = 2
        a_3 = a*3^3 + b = 5
        a_4 = a*3^4 + b = 14

        So the formula would be a_n = a*3^n + b, which is a bit different from what I said earlier.

        Let's check:
        a_1 - a_2 = a*(3^1 - 3^2) = a*3^1*(1 - 3) = -2a*3^1
        1 - 2 = -2a*3^1
        -1 = -2a*3
        a = 1/(2*3) = 1/6

        Now, using the first equation:
        1 = a*3^1 + b
        1 = 1/6 * 3 + b
        1 = 1/2 + b
        b = 1/2

        So a_n = 3^n/6 + 1/2

        But this doesn't work:
        a_1 = 3^1/6 + 1/2 = 3/6 + 1/2 = 1/2 + 1/2 = 1 ✓
        a_2 = 3^2/6 + 1/2 = 9/6 + 1/2 = 3/2 + 1/2 = 2 ✓
        a_3 = 3^3/6 + 1/2 = 27/6 + 1/2 = 9/2 + 1/2 = 5 ✓
        a_4 = 3^4/6 + 1/2 = 81/6 + 1/2 = 27/2 + 1/2 = 14 ✓

        Ah, it does work! And for a_5:
        a_5 = 3^5/6 + 1/2 = 243/6 + 1/2 = 40.5 + 0.5 = 41

        So, the next term in the sequence 1, 2, 5, 14, ... is 41.

        I think I've been making a lot of computational errors. Let me go through this one more time, methodically.

        First, let's try the direct recursive approach:
        a_1 = 1
        a_n = a_{n-1} + 3^{n-2} for n ≥ 2

        For the sequence:
        a_1 = 1 (given)
        a_2 = a_1 + 3^0 = 1 + 1 = 2 (matches)
        a_3 = a_2 + 3^1 = 2 + 3 = 5 (matches)
        a_4 = a_3 + 3^2 = 5 + 9 = 14 (matches)
        a_5 = a_4 + 3^3 = 14 + 27 = 41

        Second, let's try the direct formula approach:
        a_n = (1 + 3^{n-1})/2

        For the sequence:
        a_1 = (1 + 3^0)/2 = (1 + 1)/2 = 1 (matches)
        a_2 = (1 + 3^1)/2 = (1 + 3)/2 = 2 (matches)
        a_3 = (1 + 3^2)/2 = (1 + 9)/2 = 5 (matches)
        a_4 = (1 + 3^3)/2 = (1 + 27)/2 = 14 (matches)
        a_5 = (1 + 3^4)/2 = (1 + 81)/2 = 41

        Both methods give a_5 = 41. So the next term in the sequence 1, 2, 5, 14, ... is 41.",
                "response": "Looking at the sequence 1, 2, 5, 14, ..., I need to find the pattern to determine the next number.

        First, let me examine the differences between consecutive terms:
        - From 1 to 2: difference is 1
        - From 2 to 5: difference is 3
        - From 5 to 14: difference is 9

        I notice these differences form a pattern: 1, 3, 9, which are powers of 3: 3^0, 3^1, 3^2

        This suggests the recurrence relation:
        a₁ = 1
        aₙ = aₙ₋₁ + 3^(n-2) for n ≥ 2

        Let me verify:
        - a₁ = 1 ✓
        - a₂ = 1 + 3^0 = 1 + 1 = 2 ✓
        - a₃ = 2 + 3^1 = 2 + 3 = 5 ✓
        - a₄ = 5 + 3^2 = 5 + 9 = 14 ✓

        So for the next term:
        a₅ = 14 + 3^3 = 14 + 27 = 41

        I can also derive a direct formula. Since each term is the sum:
        aₙ = 1 + 3^0 + 3^1 + ... + 3^(n-2)

        This is 1 plus a geometric series with first term 1 and ratio 3, which simplifies to:
        aₙ = (1 + 3^(n-1))/2

        The next term is 41.",
                "performance": {
                    "time": {
                        "latency": 118.24,
                        "tpot": 0.0112,
                        "ttft": null
                    },
                    "tokens": {
                        "input_tokens": 52,
                        "cache_creation_input_tokens": 0,
                        "cache_read_input_tokens": 0,
                        "output_tokens": 10531,
                        "service_tier": "standard"
                    }
                }
            }
        }       "performance": {
            "time": {
                "latency": 118.24,
                "tpot": 0.0112,
                "ttft": null
            },
            "tokens": {
                "input_tokens": 52,
                "cache_creation_input_tokens": 0,
                "cache_read_input_tokens": 0,
                "output_tokens": 10531,
                "service_tier": "standard"
            }
        }
    }
}